Updated CSP and RPs

theories/theories/utp_csp.thy
@@ -13,6 +13,91 @@ imports
   utp_reactive
 begin
 
+definition J_pred_rea :: "'VALUE WF_PREDICATE" ("J\<^bsub>rea\<^esub>") where
+"J\<^bsub>rea\<^esub> \<equiv> (ok \<Rightarrow>p ok') \<and>p II (REL_VAR - OKAY)"
 
+syntax
+  "_upred_J_rea"        :: "upred" ("J\<^bsub>rea\<^esub>")
+
+translations
+  "_upred_J_rea"          == "CONST J_pred_rea"
+
+definition CSP1 :: "'a UTYPE \<Rightarrow> 'a WF_PREDICATE \<Rightarrow> 'a WF_PREDICATE" where
+"CSP1 a P = `P \<or> (\<not> ok \<and> (tr\<^bsub>a\<^esub> \<le> tr\<^bsub>a\<^esub>\<acute>))`"
+
+definition CSP2 :: "'a UTYPE \<Rightarrow> 'a WF_PREDICATE \<Rightarrow> 'a WF_PREDICATE" where
+"CSP2 a P = `P ; J\<^bsub>rea\<^esub>`"
+
+definition \<delta> :: "'a UTYPE \<Rightarrow> 'a WF_PREDICATE" where
+"\<delta> a = R3 a `((tr\<^bsub>a\<^esub> = tr\<^bsub>a\<^esub>\<acute>) \<and> $wait\<acute>)`"
+
+syntax 
+  "_upred_delta" :: "'a UTYPE \<Rightarrow> upred" ("\<delta>\<^bsub>_\<^esub>")
+
+translations
+  "_upred_delta a" == "CONST \<delta> a"
+
+definition STOP :: "'a UTYPE \<Rightarrow> 'a WF_PREDICATE" ("STOP\<^bsub>CSP'(_')\<^esub>") where
+"STOP\<^bsub>CSP(a)\<^esub> = CSP1 a `ok\<acute> \<and> \<delta>\<^bsub>a\<^esub>`"
+
+syntax 
+  "_upred_STOP" :: "'a UTYPE \<Rightarrow> upred" ("STOP\<^bsub>CSP'(_')\<^esub>")
+
+translations
+  "_upred_STOP a" == "CONST STOP a"
+
+definition B :: "'a UTYPE \<Rightarrow> 'a WF_PREDICATE" where
+"B a = `(tr\<^bsub>a\<^esub> = tr\<^bsub>a\<^esub>\<acute> \<and> $wait\<acute>) \<or> (tr\<^bsub>a\<^esub> \<le> tr\<^bsub>a\<^esub>\<acute>) `"
+
+syntax 
+  "_upred_B" :: "'a UTYPE \<Rightarrow> upred" ("B\<^bsub>CSP'(_')\<^esub>")
+
+translations
+  "_upred_B a" == "CONST B a"
+
+definition \<Phi> :: "'a UTYPE \<Rightarrow> 'a WF_PREDICATE \<Rightarrow> 'a WF_PREDICATE" where
+"\<Phi> a P = R a `B\<^bsub>CSP(a)\<^esub> \<and> P`"
+
+definition doA :: "'a UTYPE \<Rightarrow> 'a WF_EXPRESSION \<Rightarrow> 'a WF_PREDICATE" where
+"doA a b = \<Phi> a `((b \<notin> ref\<^bsub>a\<^esub>\<acute>)\<lhd> $wait \<rhd> (tr\<^bsub>a\<^esub>^\<langle>b\<rangle> = tr\<^bsub>a\<^esub>\<acute>))`"
+
+syntax 
+  "_upred_B" :: "'a UTYPE \<Rightarrow> 'a WF_EXPRESSION \<Rightarrow> upred" ("doA\<^bsub>CSP'(_')\<^esub>'(_')")
+
+translations
+  "_upred_B a b" == "CONST doA a b"
+
+definition prefix :: "'a WF_EXPRESSION \<Rightarrow> 'a UTYPE \<Rightarrow> 'a WF_PREDICATE" ("_\<rightarrow>\<^bsub>CSP'(_')\<^esub>SKIP") where
+"a\<rightarrow>\<^bsub>CSP(b)\<^esub>SKIP = CSP1 b `ok\<acute> \<and> doA\<^bsub>CSP(b)\<^esub>(a)`"
+
+definition SkipCSP :: "'a UTYPE \<Rightarrow> 'a WF_PREDICATE" ("SKIP\<^bsub>CSP'(_')\<^esub>") where 
+"SKIP\<^bsub>CSP(a)\<^esub> = `\<exists> ref a. II\<^bsub>rea(a)\<^esub>`"
+
+definition ChaosCSP :: "'a UTYPE \<Rightarrow> 'a WF_PREDICATE" ("CHAOS\<^bsub>CSP'(_')\<^esub>") where
+"CHAOS\<^bsub>CSP(a)\<^esub> = R a true"
+
+lemma L1 : "CHAOS\<^bsub>CSP(a)\<^esub> ; P = CHAOS\<^bsub>CSP(a)\<^esub>"
+oops
+
+lemma L2 : "STOP\<^bsub>CSP(a)\<^esub> ; P = STOP\<^bsub>CSP(a)\<^esub>"
+oops
+
+definition prefixed :: "'a WF_EXPRESSION \<Rightarrow> 'a UTYPE \<Rightarrow> 'a WF_PREDICATE \<Rightarrow> 'a WF_PREDICATE" ("_\<rightarrow>\<^bsub>CSP'(_')\<^esub>_") where
+"a\<rightarrow>\<^bsub>CSP(b)\<^esub>P = a\<rightarrow>\<^bsub>CSP(b)\<^esub>SKIP ; P"
+
+definition extchoice :: "'a WF_PREDICATE \<Rightarrow> 'a UTYPE \<Rightarrow> 'a WF_PREDICATE \<Rightarrow> 'a WF_PREDICATE" ("_\<box>\<^bsub>CSP'(_')\<^esub>_") where
+"P\<box>\<^bsub>CSP(a)\<^esub>Q = CSP2 a `((P \<and> Q)\<lhd> ((tr\<^bsub>a\<^esub> = tr\<^bsub>a\<^esub>\<acute>) \<and> $wait\<acute>) \<rhd>(P \<or> Q))`"
+
+lemma L3 : "(P \<sqinter> Q) \<box>\<^bsub>CSP(a)\<^esub> S = (P \<box>\<^bsub>CSP(a)\<^esub> S) \<sqinter> (Q \<box>\<^bsub>CSP(a)\<^esub> s)"
+oops
+
+lemma L4 : "P \<sqinter> (Q \<box>\<^bsub>CSP(a)\<^esub> S) = (P \<sqinter> Q) \<box>\<^bsub>CSP(a)\<^esub> (P \<sqinter> S)"
+oops
+
+lemma L5 : "P \<box>\<^bsub>CSP(a)\<^esub> SKIP\<^bsub>CSP(a)\<^esub> \<sqsubseteq> SKIP\<^bsub>CSP(a)\<^esub> "
+oops
+
+lemma L6sub : "((a1\<rightarrow>\<^bsub>CSP(a)\<^esub>P1) \<box>\<^bsub>CSP(a)\<^esub>  (a2\<rightarrow>\<^bsub>CSP(a)\<^esub>P2)); Q = ((a1\<rightarrow>\<^bsub>CSP(a)\<^esub>P1);Q) \<box>\<^bsub>CSP(a)\<^esub> ((a2\<rightarrow>\<^bsub>CSP(a)\<^esub>P2) ; Q)"
+oops
 
 end
